Update was easier. Don't bother with optional freeability and bolt it in

code/streaming/Hacl.Streaming.Functor.fst
@@ -6,7 +6,8 @@ module Hacl.Streaming.Functor
 /// of the index, and a type class for that index. Then, as usual, a given value
 /// for the index as a parameter.
 
-#set-options "--max_fuel 0 --max_ifuel 0"
+#set-options "--max_fuel 0 --max_ifuel 0 \
+  --using_facts_from '*,-LowStar.Monotonic.Buffer.unused_in_not_unused_in_disjoint_2' --z3rlimit 50"
 
 module ST = FStar.HyperStack.ST
 module HS = FStar.HyperStack
@@ -127,13 +128,6 @@ let optional_frame #index
       key.frame_invariant #i l s h0 h1;
       key.frame_freeable #i l s h0 h1
 
-
-let freeable #index (c: block index) (i: index) (h: HS.mem) (p: state c i (c.state.s i)) =
-  B.freeable p /\ (
-  let s = B.deref h p in
-  let State block_state buf _ _ maybe_key = s in
-  B.freeable buf /\ c.state.freeable h block_state /\ optional_freeable h maybe_key)
-
 let footprint_s #index (c: block index) (i: index) (h: HS.mem) (s: state_s c i (c.state.s i)) =
   let State block_state buf_ _ _ maybe_key = s in
   B.(loc_addr_of_buffer buf_ `loc_union` c.state.footprint h block_state `loc_union` optional_footprint h maybe_key)
@@ -170,6 +164,7 @@ let invariant_s #index (c: block index) (i: index) h (s: state_s c i (c.state.s 
   B.(loc_disjoint (loc_buffer buf_) (c.state.footprint h block_state)) /\
   B.(loc_disjoint (loc_buffer buf_) (optional_footprint h key)) /\
   B.(loc_disjoint (optional_footprint h key) (c.state.footprint h block_state)) /\
+  B.freeable buf_ /\ c.state.freeable h block_state /\ optional_freeable h key /\
 
   // Formerly, the "hashes" predicate
   S.length blocks + S.length rest = U64.v total_len /\
@@ -201,21 +196,16 @@ let frame_invariant #index c i l s h0 h1 =
   let state_t = B.deref h0 s in
   let State block_state _ _ _ maybe_key = state_t in
   c.state.frame_invariant #i l block_state h0 h1;
-  allow_inversion key_management;
-  match c.km with
-  | Erased -> ()
-  | Runtime -> c.key.frame_invariant #i l maybe_key h0 h1
-
-let frame_seen #_ _ _ _ _ _ _ =
-  ()
-
-let frame_freeable #index c i l s h0 h1 =
-  let State block_state _ _ _ maybe_key = B.deref h0 s in
   c.state.frame_freeable #i l block_state h0 h1;
   allow_inversion key_management;
   match c.km with
   | Erased -> ()
-  | Runtime -> c.key.frame_freeable #i l maybe_key h0 h1
+  | Runtime ->
+      c.key.frame_freeable #i l maybe_key h0 h1;
+      c.key.frame_invariant #i l maybe_key h0 h1
+
+let frame_seen #_ _ _ _ _ _ _ =
+  ()
 
 /// Stateful API
 /// ============
@@ -232,7 +222,6 @@ let split_at_last_empty #index (c: block index) (i: index): Lemma
 =
   ()
 
-#push-options "--using_facts_from '*,-LowStar.Monotonic.Buffer.unused_in_not_unused_in_disjoint_2' --z3rlimit 50"
 let create_in #index c i t k r =
   [@inline_let] let _ = c.state.invariant_loc_in_footprint #i in
   [@inline_let] let _ = c.key.invariant_loc_in_footprint #i in
@@ -300,7 +289,6 @@ let create_in #index c i t k r =
   (**) assert (B.fresh_loc (B.loc_addr_of_buffer p) h0 h6);
   (**) assert (B.fresh_loc (footprint_s c i h6 s) h0 h6);
   (**) c.state.frame_freeable B.loc_none block_state h5 h6;
-  (**) assert (freeable c i h6 p);
   (**) assert (optional_reveal h5 k' == optional_reveal h6 k');
 
   c.init (G.hide i) k block_state;
@@ -330,40 +318,54 @@ let create_in #index c i t k r =
   (**) assert B.(modifies loc_none h0 h8);
   (**) assert (B.fresh_loc (footprint c i h8 p) h0 h8);
   (**) assert B.(loc_includes (loc_region_only true r) (footprint c i h8 p));
-  (**) assert (freeable c i h8 p);
 
   (**) assert (ST.equal_stack_domains h1 h8);
   (**) assert (ST.equal_stack_domains h0 h1);
 
   p
-#pop-options
 
-let init #index c i t s =
-  [@inline_let]
-  let _ = c.invariant_loc_in_footprint #i in
-  [@inline_let]
-  let _ = c.frame_freeable #i in
+let init #index c i t k s =
+  [@inline_let] let _ = c.state.invariant_loc_in_footprint #i in
+  [@inline_let] let _ = c.state.frame_freeable #i in
+  [@inline_let] let _ = c.key.invariant_loc_in_footprint #i in
+  [@inline_let] let _ = c.key.frame_freeable #i in
+  allow_inversion key_management;
 
   let open LowStar.BufferOps in
-  let h1 = ST.get () in
-  let State block_state buf _ _ = !*s in
-  // JP: figuring out the alg at run-time is useful, but entails a lot more
-  // proof difficulty; note the let-binding below, as well as the fact that
-  // implicit argument resolution basically no longer works after this...
+  (**) let h1 = ST.get () in
+  let State block_state buf _ _ k' = !*s in
   let i = c.index_of_state i block_state in
   [@inline_let]
-  let block_state: c.state i = block_state in
+  let block_state: c.state.s i = block_state in
 
-  c.init (G.hide i) block_state;
-  let h2 = ST.get () in
-  c.update_multi_zero i (c.v h2 block_state);
-  split_at_last_empty c i;
+  c.init (G.hide i) k block_state;
+  (**) let h2 = ST.get () in
+  (**) optional_frame (c.state.footprint #i h1 block_state) k' h1 h2;
+  (**) c.key.frame_invariant (c.state.footprint #i h1 block_state) k h1 h2;
+  (**) c.update_multi_zero i (c.state.v i h2 block_state);
+  (**) split_at_last_empty c i;
+
+  let k': optional_key i c.km c.key =
+    match c.km with
+    | Runtime ->
+        c.key.copy i k k';
+        (**) let h4 = ST.get () in
+        (**) assert (c.key.invariant #i h4 k');
+        (**) c.key.frame_invariant (c.key.footprint #i h2 k') k h2 h4;
+        (**) c.state.frame_invariant (c.key.footprint #i h2 k') block_state h2 h4;
+        (**) c.state.frame_freeable (c.key.footprint #i h2 k') block_state h2 h4;
+        k'
+    | Erased ->
+        G.hide (c.key.v i h1 k)
+  in
+  (**) let h2 = ST.get () in
 
   [@ inline_let ]
-  let tmp: state_s c i t = State block_state buf 0UL (G.hide S.empty) in
+  let tmp: state_s c i t = State block_state buf 0UL (G.hide S.empty) k' in
   B.upd s 0ul tmp;
-  let h3 = ST.get () in
-  c.frame_invariant B.(loc_buffer s) block_state h2 h3;
+  (**) let h3 = ST.get () in
+  (**) c.state.frame_invariant B.(loc_buffer s) block_state h2 h3;
+  (**) optional_frame B.(loc_buffer s) k' h2 h3;
 
   // This seems to cause insurmountable difficulties. Puzzled.
   ST.lemma_equal_domains_trans h1 h2 h3;
@@ -371,7 +373,6 @@ let init #index c i t s =
   // AR: 07/22: same old `Seq.equal` and `==` story
   assert (Seq.equal (seen c i h3 s) Seq.empty);
 
-  assert (preserves_freeable c i s h1 h3);
   //assert (hashed h3 s == S.empty);
   assert (footprint c i h1 s == footprint c i h3 s);
   assert (B.(modifies (footprint c i h1 s) h1 h3));
@@ -380,21 +381,14 @@ let init #index c i t s =
   assert (
     let h = h3 in
     let s = B.get h3 s 0 in
-    let State block_state buf_ total_len seen = s in
+    let State block_state buf_ total_len seen _ = s in
     let seen = G.reveal seen in
     let blocks, rest = split_at_last c i seen in
-
-    // Liveness and disjointness (administrative)
-    B.live h buf_ /\ c.invariant #i h block_state /\
-    B.(loc_disjoint (loc_buffer buf_) (c.footprint #i h block_state)) /\
 
     // Formerly, the "hashes" predicate
     S.length blocks + S.length rest = U64.v total_len /\
     S.length seen = U64.v total_len /\
-    U64.v total_len < c.max_input_length i /\
-    // Note the double equals here, we now no longer know that this is a sequence.
-    c.v h block_state == c.update_multi_s i (c.init_s i) blocks /\
-    S.equal (S.slice (B.as_seq h buf_) 0 (U64.v total_len % U32.v (c.block_len i))) rest
+    U64.v total_len < c.max_input_length i
   );
   assert (invariant_s c i h3 (B.get h3 s 0))
 
@@ -454,12 +448,11 @@ let add_len #index (c: block index) (i: index) (total_len: UInt64.t) (len: UInt3
 /// We split update into several versions, to all be simplified into a single
 /// large one at extraction-time.
 
-let total_len_h #index (c: block index) (i: index) h (p: state c i (c.state i)) =
+let total_len_h #index (c: block index) (i: index) h (p: state c i (c.state.s i)) =
   State?.total_len (B.deref h p)
 
 /// Case 1: we just need to grow the buffer, no call to the hash function.
 
-#push-options "--z3rlimit 50"
 let split_at_last_small #index (c: block index) (i: index) (b: bytes) (d: bytes): Lemma
   (requires (
     let _, rest = split_at_last c i b in
@@ -525,7 +518,6 @@ let split_at_last_small #index (c: block index) (i: index) (b: bytes) (d: bytes)
   };
 
   ()
-#pop-options
 
 #push-options "--z3cliopt smt.arith.nl=false"
 let add_len_small #index (c: block index) (i: index) (total_len: UInt64.t) (len: UInt32.t): Lemma
@@ -557,7 +549,7 @@ val update_small:
   (c: block index) ->
   i:G.erased index -> (
   let i = G.reveal i in
-  t:Type0 { t == c.state i } ->
+  t:Type0 { t == c.state.s i } ->
   s:state c i t ->
   data: B.buffer uint8 ->
   len: UInt32.t ->
@@ -570,19 +562,19 @@ val update_small:
 
 #push-options "--z3rlimit 60"
 let update_small #index c i t p data len =
-  [@inline_let]
-  let _ = c.invariant_loc_in_footprint #i in
-  [@inline_let]
-  let _ = c.frame_freeable #i in
+  [@inline_let] let _ = c.state.invariant_loc_in_footprint #i in
+  [@inline_let] let _ = c.state.frame_freeable #i in
+  [@inline_let] let _ = c.key.invariant_loc_in_footprint #i in
+  [@inline_let] let _ = c.key.frame_freeable #i in
 
   let open LowStar.BufferOps in
   let h00 = ST.get () in
   assert (invariant c i h00 p);
   let s = !*p in
-  let State block_state buf total_len seen_ = s in
+  let State block_state buf total_len seen_ k' = s in
   let i = c.index_of_state i block_state in
   [@inline_let]
-  let block_state: c.state i = block_state in
+  let block_state: c.state.s i = block_state in
 
   let sz = rest c i total_len in
   add_len_small c i total_len len;
@@ -593,30 +585,30 @@ let update_small #index c i t p data len =
   B.blit data 0ul buf2 0ul len;
   let h1 = ST.get () in
   split_at_last_small c i (G.reveal seen_) (B.as_seq h0 data);
-  c.frame_invariant (B.loc_buffer buf) block_state h0 h1;
+  c.state.frame_invariant (B.loc_buffer buf) block_state h0 h1;
+  optional_frame (B.loc_buffer buf) k' h0 h1;
   assert (B.as_seq h1 data == B.as_seq h0 data);
 
   let total_len = add_len c i total_len len in
   [@inline_let]
   let tmp: state_s c i t =
-    State block_state buf total_len (G.hide (G.reveal seen_ `S.append` (B.as_seq h0 data)))
+    State #index #c #i block_state buf total_len (G.hide (G.reveal seen_ `S.append` (B.as_seq h0 data))) k'
   in
   p *= tmp;
   let h2 = ST.get () in
   assert (B.as_seq h2 data == B.as_seq h1 data);
-  c.frame_invariant (B.loc_buffer p) block_state h1 h2;
+  c.state.frame_invariant (B.loc_buffer p) block_state h1 h2;
+  optional_frame (B.loc_buffer p) k' h1 h2;
   assert (
     let b = S.append (G.reveal seen_) (B.as_seq h0 data) in
     let blocks, rest = split_at_last c i b in
     S.length blocks + S.length rest = U64.v total_len /\
     S.length b = U64.v total_len /\
     U64.v total_len <= c.max_input_length i /\
-    (==) (c.v h2 block_state) (c.update_multi_s i (c.init_s i) blocks) /\
     S.equal (S.slice (B.as_seq h2 buf) 0 (U64.v total_len % U32.v (c.block_len i))) rest
     );
   assert (seen c i h2 p `S.equal` (S.append (G.reveal seen_) (B.as_seq h0 data)));
   assert (footprint c i h0 p == footprint c i h2 p);
-  assert (preserves_freeable c i p h0 h2);
   assert (equal_domains h00 h2)
 
 #pop-options
@@ -700,7 +692,7 @@ val update_empty_buf:
   c:block index ->
   i:G.erased index -> (
   let i = G.reveal i in
-  t:Type0 { t == c.state i } ->
+  t:Type0 { t == c.state.s i } ->
   s:state c i t ->
   data: B.buffer Lib.IntTypes.uint8 ->
   len: UInt32.t ->
@@ -715,19 +707,18 @@ inline_for_extraction noextract
 let seen_pred = seen
 
 let update_empty_buf #index c i t p data len =
-  [@inline_let]
-  let _ = c.invariant_loc_in_footprint #i in
-  [@inline_let]
-  let _ = c.frame_freeable #i in
-  [@inline_let]
-  let _ = c.update_multi_associative i in
+  [@inline_let] let _ = c.state.invariant_loc_in_footprint #i in
+  [@inline_let] let _ = c.state.frame_freeable #i in
+  [@inline_let] let _ = c.key.invariant_loc_in_footprint #i in
+  [@inline_let] let _ = c.key.frame_freeable #i in
+  [@inline_let] let _ = c.update_multi_associative i in
 
   let open LowStar.BufferOps in
   let s = !*p in
-  let State block_state buf total_len seen = s in
+  let State block_state buf total_len seen k' = s in
   let i = c.index_of_state i block_state in
   [@inline_let]
-  let block_state: c.state i = block_state in
+  let block_state: c.state.s i = block_state in
   let sz = rest c i total_len in
   let h0 = ST.get () in
   assert (
@@ -741,12 +732,15 @@ let update_empty_buf #index c i t p data len =
   let data1 = B.sub data 0ul data1_len in
   let data2 = B.sub data data1_len data2_len in
   c.update_multi (G.hide i) block_state data1 data1_len;
+  let h01 = ST.get () in
+  optional_frame (c.state.footprint h0 block_state) k' h0 h01;
 
   let dst = B.sub buf 0ul data2_len in
   let h1 = ST.get () in
   B.blit data2 0ul dst 0ul data2_len;
   let h2 = ST.get () in
-  c.frame_invariant (B.loc_buffer buf) block_state h1 h2;
+  c.state.frame_invariant (B.loc_buffer buf) block_state h1 h2;
+  optional_frame (B.loc_buffer buf) k' h1 h2;
 
   S.append_assoc (G.reveal seen) (B.as_seq h0 data1) (B.as_seq h0 data2);
   assert (S.equal
@@ -754,12 +748,13 @@ let update_empty_buf #index c i t p data len =
     (S.append (G.reveal seen) (S.append (B.as_seq h0 data1) (B.as_seq h0 data2))));
 
   [@inline_let]
-  let tmp: state_s c i t = State block_state buf (add_len c i total_len len)
-    (G.hide (G.reveal seen `S.append` B.as_seq h0 data))
+  let tmp: state_s c i t = State #index #c #i block_state buf (add_len c i total_len len)
+    (G.hide (G.reveal seen `S.append` B.as_seq h0 data)) k'
   in
   p *= tmp;
   let h3 = ST.get () in
-  c.frame_invariant (B.loc_buffer p) block_state h2 h3;
+  c.state.frame_invariant (B.loc_buffer p) block_state h2 h3;
+  optional_frame (B.loc_buffer p) k' h2 h3;
 
   // After careful diagnosis, this is the difficult proof obligation that sends
   // z3 off the rails.
@@ -780,15 +775,14 @@ let update_empty_buf #index c i t p data len =
 
 
 /// Case 3: we are given just enough data to end up on the boundary
-#push-options "--z3rlimit 200"
 inline_for_extraction noextract
 val update_round:
   #index:Type0 ->
   c:block index ->
   i:G.erased index -> (
   let i = G.reveal i in
-  t:Type0 { t == c.state i } ->
-  s:state c i (c.state i) ->
+  t:Type0 { t == c.state.s i } ->
+  s:state c i (c.state.s i) ->
   data: B.buffer uint8 ->
   len: UInt32.t ->
   Stack unit
@@ -824,21 +818,20 @@ let split_at_last_block #index (c: block index) (i: index) (b: bytes) (d: bytes)
   }
 #pop-options
 
-#push-options "--z3rlimit 100"
+#push-options "--z3rlimit 200"
 let update_round #index c i t p data len =
-  [@inline_let]
-  let _ = c.invariant_loc_in_footprint #i in
-  [@inline_let]
-  let _ = c.frame_freeable #i in
-  [@inline_let]
-  let _ = c.update_multi_associative i in
+  [@inline_let] let _ = c.state.invariant_loc_in_footprint #i in
+  [@inline_let] let _ = c.state.invariant_loc_in_footprint #i in
+  [@inline_let] let _ = c.key.frame_freeable #i in
+  [@inline_let] let _ = c.key.frame_freeable #i in
+  [@inline_let] let _ = c.update_multi_associative i in
 
   let open LowStar.BufferOps in
   let s = !*p in
-  let State block_state buf_ total_len seen = s in
+  let State block_state buf_ total_len seen k' = s in
   let i = c.index_of_state i block_state in
   [@inline_let]
-  let block_state: c.state i = block_state in
+  let block_state: c.state.s i = block_state in
   let h0 = ST.get () in
   let sz = rest c i total_len in
   let diff = c.block_len i `U32.sub` sz in
@@ -850,9 +843,12 @@ let update_round #index c i t p data len =
   B.blit data 0ul buf2 0ul diff;
   let h1 = ST.get () in
   assert (S.equal (B.as_seq h1 buf0) (S.append (B.as_seq h1 buf1) (B.as_seq h1 data)));
-  c.frame_invariant (B.loc_buffer buf_) block_state h0 h1;
+  c.state.frame_invariant (B.loc_buffer buf_) block_state h0 h1;
+  c.state.frame_freeable (B.loc_buffer buf_) block_state h0 h1;
+  optional_frame (B.loc_buffer buf_) k' h0 h1;
   c.update_multi (G.hide i) block_state buf0 (c.block_len i);
   let h2 = ST.get () in
+  optional_frame (c.state.footprint h1 block_state) k' h1 h2;
   (* Proof interlude *)
   begin
     let seen' = G.reveal seen `S.append` B.as_seq h0 data in
@@ -861,38 +857,41 @@ let update_round #index c i t p data len =
     let blocks, rest = split_at_last c i seen in
     assert (S.length blocks % U32.v (c.block_len i) = 0);
     assert (S.length (rest `S.append` B.as_seq h0 data) % U32.v (c.block_len i) = 0);
+    let init = c.init_s i (optional_reveal h0 k') in
     calc (==) {
-      c.v h2 block_state;
+      c.state.v i h2 block_state;
     (==) { }
-      c.update_multi_s i (c.v h1 block_state) (B.as_seq h1 buf0);
+      c.update_multi_s i (c.state.v i h1 block_state) (B.as_seq h1 buf0);
     (==) { }
-      c.update_multi_s i (c.v h1 block_state) (B.as_seq h0 buf1 `S.append` B.as_seq h0 data);
+      c.update_multi_s i (c.state.v i h1 block_state) (B.as_seq h0 buf1 `S.append` B.as_seq h0 data);
     (==) { }
-      c.update_multi_s i (c.update_multi_s i (c.init_s i) blocks) (B.as_seq h0 buf1 `S.append` B.as_seq h0 data);
+      c.update_multi_s i (c.update_multi_s i init blocks) (B.as_seq h0 buf1 `S.append` B.as_seq h0 data);
     (==) { }
-      c.update_multi_s i (c.update_multi_s i (c.init_s i) blocks) (rest `S.append` B.as_seq h0 data);
+      c.update_multi_s i (c.update_multi_s i init blocks) (rest `S.append` B.as_seq h0 data);
     (==) { }
-      c.update_multi_s i (c.init_s i) (blocks `S.append` (rest `S.append` B.as_seq h0 data));
+      c.update_multi_s i init (blocks `S.append` (rest `S.append` B.as_seq h0 data));
     (==) { S.append_assoc blocks rest (B.as_seq h0 data) }
-      c.update_multi_s i (c.init_s i) (blocks `S.append` rest `S.append` B.as_seq h0 data);
+      c.update_multi_s i init (blocks `S.append` rest `S.append` B.as_seq h0 data);
     (==) { }
-      c.update_multi_s i (c.init_s i) (seen `S.append` B.as_seq h0 data);
+      c.update_multi_s i init (seen `S.append` B.as_seq h0 data);
     }
   end;
   [@inline_let]
-  let tmp: state_s c i t = State block_state buf_ (add_len c i total_len len)
-    (G.hide (G.reveal seen `S.append` B.as_seq h0 data))
+  let tmp: state_s c i t = State #index #c #i block_state buf_ (add_len c i total_len len)
+    (G.hide (G.reveal seen `S.append` B.as_seq h0 data)) k'
   in
   p *= tmp;
   let h3 = ST.get () in
-  c.frame_invariant (B.loc_buffer p) block_state h2 h3;
+  c.state.frame_invariant (B.loc_buffer p) block_state h2 h3;
+  c.state.frame_freeable (B.loc_buffer p) block_state h2 h3;
+  optional_frame (B.loc_buffer p) k' h2 h3;
   assert (seen_pred c i h3 p `S.equal` (S.append (G.reveal seen) (B.as_seq h0 data)))
 #pop-options
 
 let update #index c i t p data len =
   let open LowStar.BufferOps in
   let s = !*p in
-  let State block_state buf_ total_len seen = s in
+  let State block_state buf_ total_len seen k' = s in
   let i = c.index_of_state i block_state in
   let sz = rest c i total_len in
   if len `U32.lt` (c.block_len i `U32.sub` sz) then
